Now Low* Merkle tree is compiled to C

examples/low-level/merkletree/c/lib/Hacl_SHA2_256.h
@@ -1,0 +1,81 @@
+/* MIT License
+ *
+ * Copyright (c) 2016-2018 INRIA and Microsoft Corporation
+ *
+ * Permission is hereby granted, free of charge, to any person obtaining a copy
+ * of this software and associated documentation files (the "Software"), to deal
+ * in the Software without restriction, including without limitation the rights
+ * to use, copy, modify, merge, publish, distribute, sublicense, and/or sell
+ * copies of the Software, and to permit persons to whom the Software is
+ * furnished to do so, subject to the following conditions:
+ *
+ * The above copyright notice and this permission notice shall be included in all
+ * copies or substantial portions of the Software.
+ *
+ * THE SOFTWARE IS PROVIDED "AS IS", WITHOUT WARRANTY OF ANY KIND, EXPRESS OR
+ * IMPLIED, INCLUDING BUT NOT LIMITED TO THE WARRANTIES OF MERCHANTABILITY,
+ * FITNESS FOR A PARTICULAR PURPOSE AND NONINFRINGEMENT. IN NO EVENT SHALL THE
+ * AUTHORS OR COPYRIGHT HOLDERS BE LIABLE FOR ANY CLAIM, DAMAGES OR OTHER
+ * LIABILITY, WHETHER IN AN ACTION OF CONTRACT, TORT OR OTHERWISE, ARISING FROM,
+ * OUT OF OR IN CONNECTION WITH THE SOFTWARE OR THE USE OR OTHER DEALINGS IN THE
+ * SOFTWARE.
+ */
+
+
+
+#ifndef __Hacl_SHA2_256_H
+#define __Hacl_SHA2_256_H
+
+
+#include "kremlib.h"
+
+extern FStar_UInt128_uint128 FStar_Int_Cast_Full_uint64_to_uint128(uint64_t x0);
+
+extern uint32_t Hacl_SHA2_256_size_word;
+
+extern uint32_t Hacl_SHA2_256_size_hash_w;
+
+extern uint32_t Hacl_SHA2_256_size_block_w;
+
+extern uint32_t Hacl_SHA2_256_size_hash;
+
+extern uint32_t Hacl_SHA2_256_size_block;
+
+extern uint64_t Hacl_SHA2_256_max_input_len;
+
+extern uint32_t Hacl_SHA2_256_size_k_w;
+
+extern uint32_t Hacl_SHA2_256_size_ws_w;
+
+extern uint32_t Hacl_SHA2_256_size_whash_w;
+
+extern uint32_t Hacl_SHA2_256_size_count_w;
+
+extern uint32_t Hacl_SHA2_256_size_len_8;
+
+extern uint32_t Hacl_SHA2_256_size_state;
+
+extern uint32_t Hacl_SHA2_256_pos_k_w;
+
+extern uint32_t Hacl_SHA2_256_pos_ws_w;
+
+extern uint32_t Hacl_SHA2_256_pos_whash_w;
+
+extern uint32_t Hacl_SHA2_256_pos_count_w;
+
+typedef uint32_t *Hacl_SHA2_256_state;
+
+void Hacl_SHA2_256_init(uint32_t *state);
+
+void Hacl_SHA2_256_update(uint32_t *state, uint8_t *data_8);
+
+void Hacl_SHA2_256_update_multi(uint32_t *state, uint8_t *data, uint32_t n1);
+
+void Hacl_SHA2_256_update_last(uint32_t *state, uint8_t *data, uint32_t len);
+
+void Hacl_SHA2_256_finish(uint32_t *state, uint8_t *hash1);
+
+void Hacl_SHA2_256_hash(uint8_t *hash1, uint8_t *input, uint32_t len);
+
+#define __Hacl_SHA2_256_H_DEFINED
+#endif
