examples/low-level/merkletree/c/lib/connect.h
@@ -1,0 +1,4 @@
+#include "stdint.h"
+
+void MerkleTree_Low_hash_from_hashes(uint8_t *src1, uint8_t *src2, uint8_t *dst);
+
