examples/low-level/merkletree/c/merkle_tree.c
@@ -1,0 +1,25 @@
+#include "merkle_tree.h"
+#include "ext/MerkleTree_Low.h"
+
+mt_ptr create()
+{
+  return MerkleTree_Low_create_merkle_tree();
+}
+
+void insert(mt_ptr mt, hash_t v)
+{
+  MerkleTree_Low_insert(mt, v);
+}
+
+void get_root(mt_ptr mt, hash_t root)
+{
+  MerkleTree_Low_get_root(mt, root);
+}
+
+
+int main()
+{
+  /* mt_ptr mt = create(); */
+  /* hash_t elt = (hash_t )malloc(32); */
+  return 0;
+}
