examples/low-level/merkletree/c/merkle_tree.h
@@ -1,24 +1,14 @@
-// Interface
-// Assuming we have a `merkle_tree` structure
+#include "stdint.h"
+#include "ext/MerkleTree_Low.h"
 
-typedef uint8_t[32] hash_t;
-typedef uint8_t *path_t;
+typedef MerkleTree_Low_hash hash_t;
 
-typedef struct merkle_tree_s
-{
-  uint32_t nelts;
-  hash_t *values;
-  hash_t *iroots;
-}
-  merkle_tree;
-  
+typedef MerkleTree_Low_merkle_tree merkle_tree;
 typedef merkle_tree *mt_ptr;
 
 mt_ptr create();
 void insert(mt_ptr mt, hash_t v);
 void get_root(mt_ptr mt, /*output*/ hash_t root);
 
-// @param[idx]: an index of a (leaf) value in the tree
-// @return: the length of `path`
-uint32_t get_path(mt_ptr mt, uint32_t idx, /*output*/ path_t path);
-
+// tester
+int main();
